Add Simple makefile, and cleanups

proof/Simple/EvJudge.v
@@ -6,20 +6,38 @@ Require Export EsJudge.
 Require Export Exp.
 
 
-(* Big Step Evaluation **********************************************)
+(* Big Step Evaluation **********************************************
+   This is also called 'Natural Semantics'.
+ *)
 Inductive EVAL : exp -> exp -> Prop :=
- | EvValue
+ | EVValue
    :  forall v2
    ,  value v2
    -> EVAL v2 v2
 
- | EvLamApp
+ | EVLamApp
    :  forall x1 t11 x12 x2 v2 v3
    ,                              value v2               -> value v3
    -> EVAL x1 (XLam t11 x12) -> EVAL x2 v2 -> EVAL (subst v2 x12) v3
    -> EVAL (XApp x1 x2) v3.
 
 Hint Constructors EVAL.
+
+
+(* A terminating big-step evaluation always produces a value.
+   The fact that the evaluation has terminated is implied by the fact
+   that we have a proof of EVAL to pass to this lemma. If the
+   evaluation was non-terminating, then we wouldn't have a finite
+   proof of EVAL.
+ *)
+Lemma eval_produces_value
+ :  forall x1 v1
+ ,  EVAL x1 v1
+ -> value v1.
+Proof.
+ intros. destruct H; auto.
+Qed.
+Hint Resolve eval_produces_value.
 
 
 (* Big to Small steps ***********************************************)
@@ -33,7 +51,8 @@ Proof.
  induction HE.
  Case "EVValue".
   intros.
-  exists O. apply ESDone.
+  exists O.
+  apply ESDone.
 
  Case "EVLamApp".
   intros. inverts HT.
@@ -41,22 +60,11 @@ Proof.
   lets E1: IHHE1 H4. clear IHHE1. destruct E1 as [n1].
   lets E2: IHHE2 H6. clear IHHE2. destruct E2 as [n2].
 
-  lets T1: preservation_steps H4 H1. 
+  lets T1: preservation_steps H4 H1. inverts keep T1.
   lets T2: preservation_steps H6 H2.
-   inverts keep T1.
-   lets T3: subst_value_value H7 T2.
-
-  lets E3: IHHE3 T3. clear IHHE3. destruct E3 as [n3]. sort.
+  lets T3: subst_value_value H7 T2.
+  lets E3: IHHE3 T3. clear IHHE3. destruct E3 as [n3].
 
   exists (n1 + (n2 + (1 + n3))).
-  eapply ESLink.
-   eapply steps_app1. eauto.
-  eapply ESLink.
-   eapply steps_app2.
-    lets C1: type_check_empty_tyenv_is_closed T1. auto.
-   eauto.
-  eapply ESLink.
-   eapply ESStep. eapply ESLamApp.
-    auto. 
-  auto.
+   repeat (try (eapply ESLink); eauto).
 Qed.
