proof/Simple/EsJudge.v
@@ -3,7 +3,8 @@ Require Export Exp.
 Require Export SubstValueValue.
 
 
-(* Single Small Step Evaluation ************************************)
+(* Single Small Step Evaluation *************************************
+ *)
 Inductive STEP : exp -> exp -> Prop :=
  | ESLamApp
    : forall t11 x12 v2
@@ -25,17 +26,26 @@ Inductive STEP : exp -> exp -> Prop :=
 Hint Constructors STEP.
 
 
-(* Multi-step evaluation *******************************************)
+(* Multi-step evaluation *******************************************
+   This is a sequence of small step evaluations.
+ *)
 Inductive STEPS : nat -> exp -> exp -> Prop :=
+
+ (* After no steps, we get the same exp.
+    We need this constructor to match the EVValue constructor
+    in the big-step evaluation, so we can convert between big-step
+    and mult-step evaluations. *)
  | ESDone
    :  forall x1
    ,  STEPS 0 x1 x1
 
+ (* Take a single step. *)
  | ESStep
    :  forall x1 x2
    ,  STEP  x1 x2
    -> STEPS 1 x1 x2
 
+ (* Combine two reductions into a third. *)
  | ESLink
    :  forall n1 n2 x1 x2 x3
    ,  STEPS n1 x1 x2 -> STEPS n2 x2 x3
@@ -44,6 +54,10 @@ Inductive STEPS : nat -> exp -> exp -> Prop :=
 Hint Constructors STEPS.
 
 
+(* Context lemmas ***************************************************
+   These help when proving something about a reduction in a given
+   context. They're all trivial.
+ *)
 Lemma steps_app1
  :  forall n x1 x1' x2
  ,  STEPS n x1 x1'
@@ -51,6 +65,7 @@ Lemma steps_app1
 Proof.
  intros. induction H; eauto.
 Qed.
+Hint Resolve steps_app1.
 
 
 Lemma steps_app2
@@ -61,3 +76,5 @@ Lemma steps_app2
 Proof.
  intros. induction H0; eauto.
 Qed.
+Hint Resolve steps_app2.
+
